progress on BtreeBlockCache

disk-betree/BtreeBlockCache.dfy
@@ -1,17 +1,23 @@
 include "BlockCache.dfy"
 include "DiskBetree.dfy"
+include "../lib/Maps.dfy"
 
-module BtreeGraphBlockCache {
+module BetreeGraphBlockCache refines BlockCache {
   import G = BetreeGraph
 }
 
 module BtreeBlockCache {
+  import opened Maps
+
   import G = BetreeGraph
   import BC = BetreeGraphBlockCache
   import DB = DiskBetree
+  import D = Disk
 
   type Variables = BC.Variables
   type Constants = BC.Constants
+
+  type DiskOp = BC.DiskOp
 
   predicate Init(k: Constants, s: Variables) {
     BC.Init(k, s)
@@ -22,33 +28,90 @@ module BtreeBlockCache {
   }
 
   datatype Step =
-    | BetreeMoveStep(step: DB.Step)
+    | BetreeMoveStep(betreeStep: DB.Step)
+    | BlockCacheMoveStep(blockCacheStep: BC.Step)
 
-  predicate BetreeMove(k: Constants, s: Variables, s': Variables, step: DB.Step) {
-    DB.NextStep(
+  predicate BetreeMove(k: Constants, s: Variables, s': Variables, dop: DiskOp, step: DB.Step) {
+    && dop.NoDiskOp?
+    && (
+      || step.InsertMessageStep?
+      || step.FlushStep?
+      || step.GrowStep?
+      || step.SplitStep?
+    )
+    && s.Ready?
+    && s'.Ready?
+    && s' == s.(cache := s'.cache)
+    && DB.NextStep(
+        DB.Constants(DB.BI.Constants()),
+        DB.Variables(DB.BI.Variables(MapToImap(s.cache))),
+        DB.Variables(DB.BI.Variables(MapToImap(s'.cache))),
+        step)
   }
 
-  predicate NextStep(k: Constants, s: Variables, s': Variables, step: Step) {
+  predicate BlockCacheMove(k: Constants, s: Variables, s': Variables, dop: DiskOp, step: BC.Step) {
+    && (
+      || step.WriteBackStep?
+      || step.WriteBackSuperblockStep?
+      || step.UnallocStep?
+      || step.PageInStep?
+      || step.PageInSuperblockStep?
+      || step.EvictStep?
+    )
+    && BC.NextStep(k, s, s', dop, step)
+  }
+
+  predicate NextStep(k: Constants, s: Variables, s': Variables, dop: DiskOp, step: Step) {
     match step {
-      case BetreeMoveStep(step) => BetreeMove(k, s, s', step)
+      case BetreeMoveStep(step) => BetreeMove(k, s, s', dop, step)
+      case BlockCacheMoveStep(step) => BlockCacheMove(k, s, s', dop, step)
     }
   }
 
-  predicate Next(k: Constants, s: Variables, s': Variables) {
-    exists step: Step :: NextStep(k, s, s', step)
+  predicate Next(k: Constants, s: Variables, s': Variables, dop: DiskOp) {
+    exists step: Step :: NextStep(k, s, s', dop, step)
   }
 
   lemma InitImpliesInv(k: Constants, s: Variables)
   requires Init(k, s)
-  requires Inv(k, s)
+  ensures Inv(k, s)
   {
     BC.InitImpliesInv(k, s);
   }
 
-  lemma NextPreservesInv(k: Constants, s: Variables, s': Variables)
+  lemma BetreeMoveStepPreservesInv(k: Constants, s: Variables, s': Variables, dop: DiskOp, step: DB.Step)
   requires Inv(k, s)
-  requires Next(k, s, s')
-  requires Inv(k, s')
+  requires BetreeMove(k, s, s', dop, step)
+  ensures Inv(k, s')
   {
+    
+  }
+
+  lemma BlockCacheMoveStepPreservesInv(k: Constants, s: Variables, s': Variables, dop: DiskOp, step: BC.Step)
+  requires Inv(k, s)
+  requires BlockCacheMove(k, s, s', dop, step)
+  ensures Inv(k, s')
+  {
+    BC.NextStepPreservesInv(k, s, s', dop, step);
+  }
+
+  lemma NextStepPreservesInv(k: Constants, s: Variables, s': Variables, dop: DiskOp, step: Step)
+  requires Inv(k, s)
+  requires NextStep(k, s, s', dop, step)
+  ensures Inv(k, s')
+  {
+    match step {
+      case BetreeMoveStep(step) => BetreeMoveStepPreservesInv(k, s, s', dop, step);
+      case BlockCacheMoveStep(step) => BlockCacheMoveStepPreservesInv(k, s, s', dop, step);
+    }
+  }
+
+  lemma NextPreservesInv(k: Constants, s: Variables, s': Variables, dop: DiskOp)
+  requires Inv(k, s)
+  requires Next(k, s, s', dop)
+  ensures Inv(k, s')
+  {
+    var step: Step :| NextStep(k, s, s', dop, step);
+    NextStepPreservesInv(k, s, s', dop, step);
   }
 }
